Worked around bad Dafny trigger selection.  Wrote one of the two helper lemmas needed to make the top-level proof go through ( I think )

ironfleet/src/Dafny/Distributed/Services/Lock/TrueMain.i.dfy
@@ -6,12 +6,21 @@ module TrueMain_i {
     import opened QuantizedSystem_s 
 
     function LeaseSpecIoFilter(config:ConcreteConfiguration) : IoPredicate
-    {
-        (io:IoOp) -> exists epoch :: io.LIoOpReceive?
-                                  && io.r.msg == MarshallLockMsg(epoch) 
-                                  && io.r.src in config
-                                  && io.r.dst !in config
-    }
+        ensures forall io :: LeaseSpecIoFilter(config).requires(io);
+//    {
+//        (io:IoOp) -> exists epoch :: io.LIoOpReceive?
+//                                  && io.r.msg == MarshallLockMsg(epoch) 
+//                                  && io.r.src in config
+//                                  && io.r.dst !in config
+//    }
+    lemma {:axiom} LeaseSpecIoFilterDefn()
+        ensures forall config:ConcreteConfiguration, io:IoOp ::
+                    LeaseSpecIoFilter(config)(io) == 
+                             exists epoch :: io.LIoOpReceive?
+                                          && io.r.msg == MarshallLockMsg(epoch) 
+                                          && io.r.src in config
+                                          && io.r.dst !in config;
+
 
     /*
     ghost method GenerateQbToDbMapping(config:ConcreteConfiguration, qb:seq<QS_State>, db:seq<DS_State>, external_io:IoPredicate) returns (cm:seq<int>)
@@ -35,6 +44,124 @@ module TrueMain_i {
 
     }
     */
+/*
+    function ProjectExternalIOTruncated(qb:seq<QS_State>, external_io:IoPredicate, qb_index:int) : IoTrace
+        requires forall io :: external_io.requires(io);
+        requires 0 <= qb_index < |qb|;
+        reads    external_io.reads;
+        ensures  ProjectExternalIO(qb, external_io) == ProjectExternalIOTruncated(qb, external_io, qb_index) 
+                                                     + ProjectExternalIO(qb[qb_index..], external_io);
+    {
+        if qb == [] then 
+            []
+        else
+            var step := qb[0].environment.nextStep;
+            if step.LEnvStepHostIos? && |step.ios| == 1 && external_io(step.ios[0]) then
+                step.ios + 
+                    if qb_index == 0 then 
+                        []
+                    else
+                        ProjectExternalIOTruncated(qb[1..], external_io, qb_index - 1)
+            else
+                if qb_index == 0 then 
+                    []
+                else
+                    ProjectExternalIOTruncated(qb[1..], external_io, qb_index - 1)
+    }
+    */
+
+    ghost method ProjectExternalIOTruncated(qb:seq<QS_State>, external_io:IoPredicate, qb_index:int) returns (trace:IoTrace)
+        requires forall io :: external_io.requires(io);
+        requires 0 <= qb_index < |qb|;
+        ensures  ProjectExternalIO(qb, external_io) == trace
+                                                     + ProjectExternalIO(qb[qb_index+1..], external_io);
+        //ensures  qb_index > 0 ==> |trace| > 0;
+        ensures  var step := qb[qb_index].environment.nextStep;
+                 //if |trace| > 0 && step.LEnvStepHostIos? && |step.ios| == 1 && external_io(step.ios[0]) then
+                 //   last(trace) == step.ios[0]
+                 if step.LEnvStepHostIos? && |step.ios| == 1 && external_io(step.ios[0]) then
+                    |trace| > 0 && last(trace) == step.ios[0]
+                 else 
+                     true;
+    {
+        if qb == [] {
+            return [];
+        } else {
+            var step := qb[0].environment.nextStep;
+            if step.LEnvStepHostIos? && |step.ios| == 1 && external_io(step.ios[0]) {
+                if qb_index == 0 {
+                    trace := step.ios;
+                } else {
+                    var rest := ProjectExternalIOTruncated(qb[1..], external_io, qb_index - 1);
+                    trace := step.ios + rest;
+
+                    var step' := qb[1..][qb_index-1].environment.nextStep;
+                    assert qb[1..][qb_index-1] == qb[qb_index];
+                    if |rest| > 0 && step'.LEnvStepHostIos? && |step'.ios| == 1 && external_io(step'.ios[0]) { 
+                        assert last(rest) == step'.ios[0];
+                        assert last(trace) == step'.ios[0];
+                        assert last(trace) == qb[qb_index].environment.nextStep.ios[0];
+                    } else {
+                        if |rest| == 0 {
+                        } else {
+                        }
+                    }
+                }
+            } else {
+                if qb_index == 0 {
+                    trace := [];
+                } else {
+                    trace := ProjectExternalIOTruncated(qb[1..], external_io, qb_index - 1);
+                }
+            }
+        }
+    }
+
+
+
+    ghost method FindProjectExternalIOIndex(qb:seq<QS_State>, external_io:IoPredicate, qb_index:int) returns (projected_index:int)
+        requires 0 <= qb_index < |qb|;
+        requires forall io :: external_io.requires(io);
+        requires var step := qb[qb_index].environment.nextStep;
+                 step.LEnvStepHostIos? && |step.ios| == 1 && external_io(step.ios[0])
+        ensures  0 <= projected_index < |ProjectExternalIO(qb, external_io)|;
+        ensures  ProjectExternalIO(qb, external_io)[projected_index] == qb[qb_index].environment.nextStep.ios[0];
+    {
+        var truncated := ProjectExternalIOTruncated(qb, external_io, qb_index);
+        projected_index := |truncated| - 1;
+        /*
+        projected_index := 0;
+        var qb' := qb;
+        var projected_qb := [];
+        var index := 0;
+
+        while index < qb_index 
+            invariant 0 <= index <= qb_index;
+            invariant |projected_qb| <= index;
+            invariant |qb'| == |qb| - index;
+            invariant index == qb_index ==> |projected_qb| >= 1;
+            invariant ProjectExternalIO(qb, external_io) == projected_qb + ProjectExternalIO(qb', external_io);
+        {
+            var step := qb'[0].environment.nextStep;
+            if step.LEnvStepHostIos? && |step.ios| == 1 && external_io(step.ios[0]) {
+                projected_qb := projected_qb + step.ios;
+            }
+            qb' := qb'[1..];
+
+            index := index + 1;
+        }
+
+        projected_index := |projected_qb| - 1;
+        */
+    }
+
+    ghost method FindProjectDsExternalIOIndex(db:seq<DS_State>, external_io:IoPredicate, projected_index:int) returns (db_index:int)
+        requires 0 <= db_index < |db|;
+        requires forall io :: external_io.requires(io);
+        requires var step := db[db_index].environment.nextStep;
+                 step.LEnvStepHostIos? && |step.ios| == 1 && external_io(step.ios[0])
+        ensures  0 <= projected_index < |ProjectDsExternalIO(db, external_io)|;
+        ensures  ProjectDsExternalIO(db, external_io)[projected_index] == db[db_index].environment.nextStep.ios[0];
 
     lemma UltimateRefinementProof(config:ConcreteConfiguration, qb:seq<QS_State>) returns (sb:seq<ServiceState>)
         requires |qb| > 0;
@@ -48,31 +175,28 @@ module TrueMain_i {
                       && (forall i :: 0 <= i < |io_partition| ==> HostNext(behavior[i], behavior[i+1], io_partition[i])); 
         ensures  |qb| == |sb|;
         ensures  Service_Init(sb[0], Collections__Maps2_s.mapdomain(qb[0].servers));
-        //ensures  forall i {:trigger Service_Next(sb[i], sb[i+1])} :: 0 <= i < |sb| - 1 ==> (sb[i] == sb[i+1]) || Service_Next(sb[i], sb[i+1]);
-        //ensures  forall i :: 0 <= i < |qb| ==> Service_Correspondence(qb[i].environment.nextStep, sb[i]);
+        ensures  forall i {:trigger Service_Next(sb[i], sb[i+1])} :: 0 <= i < |sb| - 1 ==> (sb[i] == sb[i+1]) || Service_Next(sb[i], sb[i+1]);
+        ensures  forall i :: 0 <= i < |qb| ==> Service_Correspondence(qb[i].environment.nextStep, sb[i]);
     {
         var qb', db' := BryansProof(config, qb, LeaseSpecIoFilter); 
 
         sb := RefinementProof(config, db');
 
-        calc ==> {
-            true;
-            Service_Init(sb[0], Collections__Maps2_s.mapdomain(db'[0].servers));
-            Service_Init(sb[0], Collections__Maps2_s.mapdomain(qb'[0].servers));
-            Service_Init(sb[0], Collections__Maps2_s.mapdomain(qb[0].servers));
-        }
-        assert |qb| == |sb|;
-
-        assert Service_Init(sb[0], Collections__Maps2_s.mapdomain(qb[0].servers));        
-
         forall i {:trigger Service_Correspondence(qb[i].environment.nextStep, sb[i])} | 0 <= i < |qb| 
           ensures Service_Correspondence(qb[i].environment.nextStep, sb[i]);
         {
-          assume false;
+          assert Service_Correspondence(db'[i].environment.nextStep, sb[i]);
+          LeaseSpecIoFilterDefn();
+
+          var step := qb[i].environment.nextStep;
+          if step.LEnvStepHostIos? && |step.ios| == 1 && LeaseSpecIoFilter(config)(step.ios[0]) {
+            
+            var projected_index := FindProjectExternalIOIndex(qb, LeaseSpecIoFilter(config), i); 
+            assert Service_Correspondence(qb[i].environment.nextStep, sb[i]);
+          } else {
+            assert Service_Correspondence(qb[i].environment.nextStep, sb[i]);
+          }
+          assert Service_Correspondence(qb[i].environment.nextStep, sb[i]);
         }
-
-        
-
-
     }
 }
